examples/pseudo_bool/cp_encoding/array/cpProgScript.sml
@@ -688,25 +688,23 @@ val res = translate cp_to_ilp_schedulingTheory.cumul_contrib_ge_def;
 val res = translate cp_to_ilp_schedulingTheory.cumul_contrib_le_def;
 val res = translate cp_to_ilp_schedulingTheory.cumul_contrib_le0_def;
 val res = translate cp_to_ilp_schedulingTheory.mk_cumul_active_def;
-val res = translate cp_to_ilp_schedulingTheory.cumul_tlo_def;
-val res = translate cp_to_ilp_schedulingTheory.cumul_thi_def;
+val res = translate cp_to_ilp_schedulingTheory.task_lo_def;
+val res = translate cp_to_ilp_schedulingTheory.task_hi_def;
+val res = translate cp_to_ilp_schedulingTheory.cumul_covers_def;
+val res = translate cp_to_ilp_schedulingTheory.cumul_ts_task_def;
+
+Theorem cumul_ts_task_side[local]:
+  cumul_ts_task_side a b c ⇔ T
+Proof
+  rw[fetch "-" "cumul_ts_task_side_def"]>>intLib.ARITH_TAC
+QED
+val _ = update_precondition cumul_ts_task_side;
+
+val res = translate cp_to_ilp_schedulingTheory.cumul_times_def;
 val res = translate cp_to_ilp_schedulingTheory.mk_cumul_contrib_def;
 val res = translate cp_to_ilp_schedulingTheory.cumul_nonneg_def;
 val res = translate cp_to_ilp_schedulingTheory.cumul_cap_line_def;
 val res = translate cp_to_ilp_schedulingTheory.cencode_cumulative_def;
-
-Theorem cencode_cumulative_side[local]:
-  cencode_cumulative_side a b c d e f ⇔ T
-Proof
-  rw[fetch "-" "cencode_cumulative_side_def"]>>
-  `cumul_tlo a (ZIP (b,ZIP (c,d))) ≤ 0` by
-    simp[cp_to_ilp_schedulingTheory.cumul_tlo_LE_0]>>
-  `0 ≤ cumul_thi a (ZIP (b,ZIP (c,d)))` by
-    simp[cp_to_ilp_schedulingTheory.cumul_thi_0_LE]>>
-  rpt(qpat_x_assum`LENGTH _ = LENGTH _`kall_tac)>>
-  intLib.ARITH_TAC
-QED
-val _ = update_precondition cencode_cumulative_side;
 
 val res = translate cp_to_ilp_schedulingTheory.cencode_scheduling_constr_def;
 
